ch5

TransitionSystems_template.v
@@ -4,6 +4,7 @@
   * License: https://creativecommons.org/licenses/by-nc-nd/4.0/ *)
 
 Require Import Frap.
+Require Import Program.Equality.
 
 Set Implicit Arguments.
 (* This command will treat type arguments to functions as implicit, like in
@@ -25,6 +26,10 @@ Inductive fact_state :=
 | WithAccumulator (input accumulator : nat).
 
 (* *Initial* states *)
+(* PREDICATE. 
+ - parameters (before main colon): stay fixed throughout rec invoc of pred
+ - followed by type expressing additional args, followed by [Prop]
+*)
 Inductive fact_init (original_input : nat) : fact_state -> Prop :=
 | FactInit : fact_init original_input (WithAccumulator original_input 1).
 
@@ -45,9 +50,92 @@ Inductive fact_step : fact_state -> fact_state -> Prop :=
 Inductive trc {A} (R : A -> A -> Prop) : A -> A -> Prop :=
 | TrcRefl : forall x, trc R x x
 | TrcFront : forall x y z,
-  R x y
-  -> trc R y z
-  -> trc R x z.
+  R x y -> trc R y z
+    -> trc R x z.
+
+Print True.
+Print False.
+ 
+Inductive isZero : nat -> Prop :=
+| IsZero : isZero 0.
+Theorem isZero_contra : isZero 1 -> False.
+Proof.
+  destruct 1.
+  Undo.
+  (* restriction in tactics like destruct and induction when applied to types with arguments:
+   * If the arguments are not already free variables, they will be replaced by new free 
+   * variables internally before doing the case analysis or induction.
+   * "logically complete case analysis" is undecidable in Coq logic. *)
+   intro. inversion H. (* inversion 1. *)
+   (* Think of it as a version of destruct that does its best to take advantage of
+    * the structure of arguments to inductive types. 
+    * In this case, using isZero with an impossible argument -> done *)
+Qed.
+
+
+(* induction on Prop. 
+http://www.cs.cornell.edu/~clarkson/courses/csci6907/2014sp/terse/MoreInd.html
+http://www.cs.cornell.edu/~clarkson/courses/csci6907/2014sp/sf/ProofObjects.html
+*)
+
+Print le.
+Check le_ind.
+
+
+(* [dependent induction]
+ * From an instantiated inductive predicate and a goal, it generates an
+ * equivalent goal where the hypothesis has been generalized over its ^indexes^
+ * which are then constrained by equalities to be the right instances. 
+ *)
+Lemma le_minus : forall n:nat, n < 1 -> n = 0.
+Proof.
+  intros n H. induction H. (* lose info on hypo instance *)
+  Undo.
+  dependent induction H.
+  reflexivity.
+  inversion H.
+Qed.
+
+(* 5.7 *)
+Check trc_ind.
+Theorem trc_trans : forall {A} (R : A -> A -> Prop) x y z,
+  trc R x y ->  trc R y z -> trc R x z.
+Proof.
+(*
+  simplify.
+  dependent induction H. (* rule induction? *)
+*)
+(*
+trc_ind
+     : forall (A : Type) (R P : A -> A -> Prop),
+       (forall x : A, P x x) ->
+       (forall x y z : A, R x y -> trc R y z -> P y z -> P x z) ->
+       forall y y0 : A, trc R y y0 -> P y y0
+ 
+  match goal with
+    | [ |- forall x : ?E, _ ] => (* forall x ????????????*)
+      match type of E with
+      | Prop => let H := fresh in intro H; induct H
+      end
+    | _ => intro end.
+*)
+  (* induct 1. simplify.  induction on 1st ^hypothesis^ *)
+
+  simplify. induct H.
+  (* rule induction on derivation of [trc R x y] *)
+  assumption.
+  
+  (*apply TrcFront. ** Error: Unable to find an instance for the variable y.*)
+  eapply TrcFront.
+  (*behaves like apply but it does not fail when no instantiations are deducible
+    for some variables in the premises. Rather, it turns these variables into 
+    ^existential^ variables which are variables still to instantiate. *)
+  eassumption. (* instantiation *)
+  
+  apply IHtrc.
+  assumption.
+Qed.
+  
 
 (* Transitive-reflexive closure is so common that it deserves a shorthand notation! *)
 Notation "R ^*" := (trc R) (at level 0).
@@ -55,7 +143,24 @@ Notation "R ^*" := (trc R) (at level 0).
 (* Now let's use it to execute the factorial program. *)
 Example factorial_3 : fact_step^* (WithAccumulator 3 1) (AnswerIs 6).
 Proof.
-Admitted.
+(*
+  eapply TrcFront.
+  apply FactStep.
+  simplify.
+  eapply TrcFront.
+  apply FactStep.
+  simplify.
+  eapply TrcFront.
+  apply FactStep.
+  simplify.
+  eapply TrcFront.
+  apply FactDone.
+  apply TrcRefl.
+*)
+  repeat econstructor.
+  (* try all declared rules of pred in concl, attempting each with eapply until it works *)
+Qed.
+
 
 (* It will be useful to give state machines more first-class status, as
  * *transition systems*, formalized by this record type.  It has one type
@@ -64,6 +169,7 @@ Record trsys state := {
   Initial : state -> Prop;
   Step : state -> state -> Prop
 }.
+Check Initial.
 
 (* The example of our factorial program: *)
 Definition factorial_sys (original_input : nat) : trsys fact_state := {|
@@ -88,8 +194,9 @@ Definition invariantFor {state} (sys : trsys state) (invariant : state -> Prop) 
 (* That is, when we begin in an initial state and take any number of steps, the
  * place we wind up always satisfies the invariant. *)
 
+
 (* Here's a simple lemma to help us apply an invariant usefully,
- * really just restating the definition. *)
+ * really just restating the definition. -> ??*)
 Lemma use_invariant' : forall {state} (sys : trsys state)
   (invariant : state -> Prop) s s',
   invariantFor sys invariant
@@ -103,6 +210,17 @@ Proof.
   eassumption.
   assumption.
 Qed.
+
+(*
+invariantFor
+     : trsys ?state -> (?state -> Prop) -> Prop
+use_invariant'
+     : forall (sys : trsys ?state) (invariant : ?state -> Prop)
+         (s s' : ?state),
+       invariantFor sys invariant ->
+       Initial sys s -> (Step sys) ^* s s' -> invariant s'
+where ?state : [ |- Type] *)
+
 
 Theorem use_invariant : forall {state} (sys : trsys state)
   (invariant : state -> Prop) s,
@@ -126,9 +244,8 @@ Lemma invariant_induction' : forall {state} (sys : trsys state)
      -> invariant s
      -> invariant s'.
 Proof.
+  (* intro. intro. intro. intro. intro. intro. intro. induct H0. *)
   induct 2; propositional.
-  (* [propositional]: simplify the goal according to the rules of propositional
-   *   logic. *)
 
   apply IHtrc.
   eapply H.
@@ -151,13 +268,32 @@ Proof.
 Qed.
 
 Definition fact_invariant (original_input : nat) (st : fact_state) : Prop :=
-  True.
-(* We must fill in a better invariant. *)
+  match st with
+  | AnswerIs ans => fact original_input = ans
+  | WithAccumulator n acc => fact original_input = fact n * acc
+  end.
 
 Theorem fact_invariant_ok : forall original_input,
   invariantFor (factorial_sys original_input) (fact_invariant original_input).
 Proof.
-Admitted.
+  simplify.
+  apply invariant_induction; simplify.
+  
+  (* Base case: invar holds at the start *)
+  (* H: fact_init original_input s -> can fraw concl about what [s] must be. *)
+  inversion H; clear H; subst. (* invert H. *)
+  simplify; ring.
+  
+  (* Ind Step: Steps preserve the invar *)
+  invert H0. 
+  Print fact_step.
+  simplify; linear_arithmetic.
+  
+  simplify.
+  rewrite H.
+  ring.
+Qed.  
+
 
 (* Therefore, every reachable state satisfies this invariant. *)
 Theorem fact_invariant_always : forall original_input s,
@@ -175,7 +311,10 @@ Lemma fact_ok' : forall original_input s,
   fact_final s
   -> fact_invariant original_input s
   -> s = AnswerIs (fact original_input).
-Admitted.
+Proof.
+  invert 1; simplify. equality.
+Qed.
+
 
 Theorem fact_ok : forall original_input s,
   reachable (factorial_sys original_input) s
@@ -278,6 +417,7 @@ Inductive parallel_init shared private1 private2
   init1 {| Shared := sh; Private := pr1 |}
   -> init2 {| Shared := sh; Private := pr2 |}
   -> parallel_init init1 init2 {| Shared := sh; Private := (pr1, pr2) |}.
+Check Pinit.
 
 Inductive parallel_step shared private1 private2
           (step1 : threaded_state shared private1 -> threaded_state shared private1 -> Prop)
@@ -307,17 +447,70 @@ Definition increment2_sys := parallel increment_sys increment_sys.
 
 (* Let's prove that the counter is always 2 when the composed program terminates. *)
 
+(* 1. PC of thread tells how much it has added to the shared counter *)
+Definition contribution_from (pr : increment_program) : nat :=
+  match pr with
+  | Unlock | Done => 1
+  | _ => 0
+  end.
+
+(* 2. PC also tells whether a thread holds the lock *)
+Definition has_lock (pr : increment_program) : bool :=
+  match pr with
+  | Read | Write _ | Unlock => true
+  | _ => false
+  end.
+
+(* shared state = func of 2 PCs *)
+Definition shared_from_private (pr1 pr2 : increment_program) :=
+  {| Locked := has_lock pr1 || has_lock pr2
+   ; Global := contribution_from pr1 + contribution_from pr2
+  |}.
+
+(* compatibility b/w PCs. e.g. shouldn't both be in critical section at once *)
+Definition instruction_ok (self other : increment_program): Prop :=
+  match self with
+  | Lock => True
+  | Read | Unlock => has_lock other = false
+  | Write n => has_lock other = false /\ n = contribution_from other
+  | Done => True
+  end. 
+
 (** We must write an invariant. *)
 Inductive increment2_invariant :
   threaded_state inc_state (increment_program * increment_program) -> Prop :=
-| Inc2Inv : forall sh pr1 pr2,
-  increment2_invariant {| Shared := sh; Private := (pr1, pr2) |}.
-(* This isn't it yet! *)
+| Inc2Inv : forall pr1 pr2,
+  instruction_ok pr1 pr2
+  -> instruction_ok pr2 pr1
+  -> increment2_invariant {| Shared := shared_from_private pr1 pr2; Private := (pr1, pr2) |}.
+
+(* Convenient to prove alternative _equality-based_ constructor for the invariant *)
+Lemma Inc2Inv' : forall sh pr1 pr2,
+  sh = shared_from_private pr1 pr2
+  -> instruction_ok pr1 pr2
+  -> instruction_ok pr2 pr1
+  -> increment2_invariant {| Shared := sh; Private := (pr1, pr2) |}.
+Proof.
+  simplify.
+  rewrite H.
+  apply Inc2Inv; assumption.
+Qed.
+Print Inc2Inv'. (* function value = proof *)
 
 (* Now, to show it really is an invariant. *)
 Theorem increment2_invariant_ok : invariantFor increment2_sys increment2_invariant.
 Proof.
-Admitted.
+  apply invariant_induction; simplify;
+  repeat match goal with
+         | [ H : increment2_invariant _ |- _ ] => invert H
+         | [ H : parallel_init _ _ _ |- _] => invert H
+         | [ H : increment_init _ |- _] => invert H
+         | [ H : parallel_step _ _ _ _ |- _ ] => invert H
+         | [ H : increment_step _ _ |- _ ] => invert H
+         | [ pr : increment_program |- _ ] => cases pr; simplify
+         end; try equality;
+  apply Inc2Inv'; unfold shared_from_private; simplify; equality.
+Qed.
 
 (* Now, to prove our final result about the two incrementing threads, let's use
  * a more general fact, about when one invariant implies another. *)
@@ -346,23 +539,17 @@ Theorem increment2_sys_correct : forall s,
   reachable increment2_sys s
   -> increment2_right_answer s.
 Proof.
-Admitted.
-(*simplify.
+  simplify.
   eapply use_invariant.
   apply invariant_weaken with (invariant1 := increment2_invariant).
-  (* Note the use of a [with] clause to specify a quantified variable's
-   * value. *)
-
+  
   apply increment2_invariant_ok.
-
+  
   simplify.
   invert H0.
   unfold increment2_right_answer; simplify.
-  invert H0.
-  (* Here we use inversion on an equality, to derive more primitive
-   * equalities. *)
-  simplify.
-  equality.
-
+  invert H0. (* H0 : (pr1, pr2) = (Done, Done) *)
+  simplify; equality.
+  
   assumption.
-Qed.*)
+Qed.
